\ifdefined\MASTERDOCUMENT
\else
\documentclass{article}
\input{header}
\begin{document}

Derivations of $\D{\ln x}{x}$



1. Using the definition of derivative

\begin{eqnarray*}
  \D{f}{x} & = & \lim_{h \to 0} \frac{f(x+h)-f(x)}{h} \\ 
  \D{\ln x}{x} & = & \lim_{h \to 0} \frac{\ln(x+h)-\ln(x)}{h} \\ 
  \text{Using difference property of $\ln$ logarthms} \\
  & = & \lim_{h \to 0} \frac{1}{h}\ln(\frac{x+h}{x}) \\ 
  & = & \lim_{h \to 0} \ln\left(\frac{x+h}{x}\right)^{\frac{1}{h}} \\ 
  & = & \lim_{h \to 0} \ln\left(1 + \frac{h}{x}\right)^{\frac{1}{h}} \\ 
\text{Substitute $u = \frac{x}{h}$ } \\
   & = & \lim_{h \to 0} \ln\left(1 + \frac{1}{u}\right)^{\frac{u}{x}} \\ 
   & = & \lim_{h \to 0} \ln\left(\left(1 + \frac{1}{u}\right)^{u}\right)^{\frac{1}{x}} \\
   & = & \lim_{h \to 0} \ln\left(e)^{\frac{1}{x}} \\
   & = & \lim_{h \to 0} \frac{1}{x} \\
   & = & \frac{1}{x} \\
\end{eqnarray*}



2. Use implicit differentiataion

Start with the idea that we do know the derivative of $e^y$.
\begin{eqnarray*}
  e^y &= & x \\
  \D{e^y}{x} & = & \D{}{x}x \\

\end{eqnarray*}






\fi
\ifdefined\MASTERDOCUMENT
\endinput
\else
\expandafter\enddocument
\fi
